Delay building of L3 equivalence proofs until needed

compiler/encoders/arm8_asl/arm8_asl_targetScript.sml
@@ -2,11 +2,12 @@
   Define the target compiler configuration for ASL-derived ARMv8.
 *)
 open HolKernel Parse boolLib bossLib;
-open asmLib arm8_targetTheory l3_equivalenceTheory;
+open asmLib arm8_targetTheory armv86a_terminationTheory;
 
 val _ = new_theory "arm8_asl_target";
 
 val _ = wordsLib.guess_lengths();
+val _ = monadsyntax.enable_monad "sail2_state_monad";
 
 (********** Next-state function **********)
 
@@ -30,7 +31,6 @@ Definition arm8_asl_next_def:
   od
 End
 
-
 (********** Valid states **********)
 
 Definition arm8_asl_mem_ok_def:
@@ -47,14 +47,27 @@ End
 
 Definition arm8_asl_ok_def:
   arm8_asl_ok asl ⇔
-    asl_sys_regs_ok asl ∧
     (PSTATE_ref.read_from asl.regstate).ProcState_EL = 0w ∧ (* EL0 *)
     ¬word_bit 4 (SCTLR_EL1_ref.read_from asl.regstate) ∧ (* ¬SCTLR_EL1.SA0 *)
     ¬word_bit 24 (SCTLR_EL1_ref.read_from asl.regstate) ∧ (* ¬SCTLR_EL1.EOE *)
     ¬word_bit 37 (TCR_EL1_ref.read_from asl.regstate) ∧ (* ¬TCR_EL1.TBI0 *)
     ¬word_bit 38 (TCR_EL1_ref.read_from asl.regstate) ∧ (* ¬TCR_EL1.TBI1 *)
     aligned 2 (PC_ref.read_from asl.regstate) ∧ (* aligned 2 PC *)
-    arm8_asl_mem_ok asl ∧ arm8_asl_regs_ok asl
+    arm8_asl_mem_ok asl ∧ arm8_asl_regs_ok asl ∧
+
+    ¬(highest_el_aarch32_ref.read_from asl.regstate) ∧
+    (PSTATE_ref.read_from asl.regstate).ProcState_nRW = 0w ∧
+    word_bit 0 (SCR_EL3_ref.read_from asl.regstate) ∧
+    word_bit 10 (SCR_EL3_ref.read_from asl.regstate) ∧
+    ¬word_bit 18 (SCR_EL3_ref.read_from asl.regstate) ∧
+    word_bit 31 (HCR_EL2_ref.read_from asl.regstate) ∧
+    ¬word_bit 34 (HCR_EL2_ref.read_from asl.regstate) ∧
+    CNTControlBase_ref.read_from asl.regstate = 0w ∧
+    word_bit 4 ((PSTATE_ref.read_from asl.regstate).ProcState_M) ∧
+    ¬word_bit 51 (TCR_EL1_ref.read_from asl.regstate) ∧
+    ¬word_bit 52 (TCR_EL1_ref.read_from asl.regstate) ∧
+    ¬word_bit 29 (TCR_EL2_ref.read_from asl.regstate) ∧
+    ¬word_bit 29 (TCR_EL3_ref.read_from asl.regstate)
 End
 
 (********** Target record **********)
@@ -67,7 +80,19 @@ Definition arm8_asl_proj_def:
     R_ref.read_from asl.regstate,
     fun2set ($' asl.memstate o w2n, mem),
     PC_ref.read_from asl.regstate,
-    asl_sys_regs_ok asl,
+      ¬(highest_el_aarch32_ref.read_from asl.regstate) ∧
+      (PSTATE_ref.read_from asl.regstate).ProcState_nRW = 0w ∧
+      word_bit 0 (SCR_EL3_ref.read_from asl.regstate) ∧
+      word_bit 10 (SCR_EL3_ref.read_from asl.regstate) ∧
+      ¬word_bit 18 (SCR_EL3_ref.read_from asl.regstate) ∧
+      word_bit 31 (HCR_EL2_ref.read_from asl.regstate) ∧
+      ¬word_bit 34 (HCR_EL2_ref.read_from asl.regstate) ∧
+      CNTControlBase_ref.read_from asl.regstate = 0w ∧
+      word_bit 4 ((PSTATE_ref.read_from asl.regstate).ProcState_M) ∧
+      ¬word_bit 51 (TCR_EL1_ref.read_from asl.regstate) ∧
+      ¬word_bit 52 (TCR_EL1_ref.read_from asl.regstate) ∧
+      ¬word_bit 29 (TCR_EL2_ref.read_from asl.regstate) ∧
+      ¬word_bit 29 (TCR_EL3_ref.read_from asl.regstate),
     arm8_asl_mem_ok asl,
     arm8_asl_regs_ok asl
     )
